test/AssocList.fst
@@ -1,0 +1,46 @@
+module AssocList
+
+/// Testing the API of the interactive map
+
+module I = LowStar.Lib.AssocList
+module M = FStar.Map
+module B = LowStar.Buffer
+module HS = FStar.HyperStack
+module ST = FStar.HyperStack.ST
+
+open LowStar.BufferOps
+open FStar.HyperStack.ST
+
+#set-options "--fuel 0 --ifuel 0"
+
+let main (): St unit =
+  let r = ST.new_region HS.root in
+  let m: I.t nat (nat & nat) = I.create_in r in
+  (**) let h0 = ST.get () in
+  (**) assert (M.sel (I.v h0 m) 0 == None);
+  I.add m 0 (1, 2);
+  (**) let h1 = ST.get () in
+  (**) assert (M.sel (I.v h1 m) 0 == Some (1, 2));
+  let b = B.malloc HS.root 0ul 1ul in
+  (**) let h2 = ST.get () in
+  (**) assert (M.sel (I.v h2 m) 0 == Some (1, 2));
+  b *= 2ul;
+  (**) let h3 = ST.get () in
+  (**) assert B.(loc_disjoint (loc_buffer b) (I.footprint h3 m));
+  (**) assert (M.sel (I.v h3 m) 0 == Some (1, 2));
+  I.add m 0 (2, 1);
+  (**) let h4 = ST.get () in
+  (**) assert (M.sel (I.v h4 m) 0 == Some (2, 1));
+  (**) assert (B.deref h4 b == 2ul);
+  (**) I.footprint_in_r h4 m; // FIXME
+  (**) assert B.(loc_disjoint (loc_buffer b) (I.footprint h4 m));
+  I.remove_all m 1;
+  (**) let h5 = ST.get () in
+  (**) assert (M.sel (I.v h5 m) 0 == Some (2, 1));
+  (**) assert (B.deref h5 b == 2ul);
+  (**) I.footprint_in_r h5 m; // FIXME
+  I.remove_all m 0;
+  (**) let h6 = ST.get () in
+  (**) assert (M.sel (I.v h6 m) 0 == None);
+  (**) assert (B.deref h6 b == 2ul);
+  ()
